src/cbor/pulse/CBOR.Pulse.API.Det.Type.fsti
@@ -2,3 +2,5 @@ module CBOR.Pulse.API.Det.Type
 
 val cbor_det_t: Type0
 val cbor_det_map_entry_t: Type0
+val cbor_det_array_iterator_t: Type0
+val cbor_det_map_iterator_t: Type0
